WIP: canonicalising resources

ulib/FStar.Tactics.CanonCommMonoidSimple.Equiv.fst
@@ -287,12 +287,6 @@ let monoid_reflect (#a:Type) (eq:equiv a) (m:cm a eq) (am:amap a) (e1 e2:exp)
        : squash (mdenote eq m am e1 `EQ?.eq eq` mdenote eq m am e2) =
   monoid_reflect_orig #a eq m am e1 e2
 
-let monoid_reflexivity (#a:Type) (eq:equiv a) (m:cm a eq) (am:amap a) (e:exp)
-  : squash ((let FStar.Algebra.CommMonoid.Equiv.EQ eq _ _ _ = 
-               eq in
-              eq) (mdenote eq m am e) (mdenote eq m am e)) =
-  EQ?.reflexivity eq (mdenote eq m am e)
-
 (* Finds the position of first occurrence of x in xs.
    This is now specialized to terms and their funny term_eq. *)
 let rec where_aux (n:nat) (x:term) (xs:list term) :
@@ -333,6 +327,129 @@ let reification (#a:Type) (eq:equiv a) (m:cm a eq) (ts:list term) (am:amap a) (t
 
 let canon_monoid (#a:Type) (eq:equiv a) (m:cm a eq) : Tac unit =
   norm [];
+  let t = cur_goal () in 
+  // removing top-level squash application
+  let sq, rel_xy = collect_app_ref t in
+  // unpacking the application of the equivalence relation (lhs `EQ?.eq eq` rhs)
+  (match list_unref rel_xy with
+   | [(rel_xy,_)] -> (
+       let rel, xy = collect_app_ref rel_xy in
+       match list_unref xy with 
+       // when the relation takes zero implicit arguments
+       | [(lhs, Q_Explicit) ; (rhs, Q_Explicit)] -> (
+           let (r1, ts, am) = reification eq m [] (const (CM?.unit m)) lhs in
+           let (r2, _, am) = reification eq m ts am rhs in
+           //dump ("am = " ^ term_to_string (quote am));
+           dump ("before = " ^ term_to_string (norm_term [hnf;delta;primops]
+              (quote (mdenote eq m am r1 `EQ?.eq eq` mdenote eq m am r2)))); 
+           //dump ("current goal" ^ term_to_string (cur_goal ()));
+           change_sq (quote (mdenote eq m am r1 `EQ?.eq eq` mdenote eq m am r2));
+           //dump ("expected after = " ^ term_to_string (norm_term [delta;primops]
+           //   (quote (xsdenote eq m am (canon r1) `EQ?.eq eq`
+           //           xsdenote eq m am (canon r2)))));
+           apply (`monoid_reflect);
+           //dump ("after apply");
+           norm [delta_only [`%canon; `%xsdenote; `%flatten; `%sort;
+                             `%select; `%assoc; `%fst; `%__proj__Mktuple2__item___1;
+                             `%(@); `%append; `%List.Tot.Base.sortWith;
+                             `%List.Tot.Base.partition; `%bool_of_compare; 
+                             `%compare_of_bool; //`%EQ?.eq;
+                ]; primops]
+           //;dump "after norm"
+         )
+       // when the relation takes one implicit argument
+       | [_ ; (lhs, Q_Explicit) ; (rhs, Q_Explicit)] -> (
+           let (r1, ts, am) = reification eq m [] (const (CM?.unit m)) lhs in
+           let (r2, _, am) = reification eq m ts am rhs in
+           //dump ("am = " ^ term_to_string (quote am));
+           change_sq (quote (mdenote eq m am r1 `EQ?.eq eq` mdenote eq m am r2));
+           //dump ("before = " ^ term_to_string (norm_term [delta;primops]
+           //   (quote (mdenote eq m am r1 `EQ?.eq eq` mdenote eq m am r2)))); 
+           //dump ("expected after = " ^ term_to_string (norm_term [delta;primops]
+           //   (quote (xsdenote eq m am (canon r1) `EQ?.eq eq`
+           //           xsdenote eq m am (canon r2)))));
+           apply (`monoid_reflect);
+           //dump ("after apply");
+           norm [delta_only [`%canon; `%xsdenote; `%flatten; `%sort;
+                             `%select; `%assoc; `%fst; `%__proj__Mktuple2__item___1;
+                             `%(@); `%append; `%List.Tot.Base.sortWith;
+                             `%List.Tot.Base.partition; `%bool_of_compare; 
+                             `%compare_of_bool; //`%EQ?.eq;
+                ]; primops]
+           //;dump "after norm"
+         )
+       | _ -> fail "Goal should be a binary relation"
+     )
+   | _ -> fail "Goal should be squash applied to a binary relation")
+
+(***** Example *)
+
+(*
+let test1 (a b c d : int) =
+  assert_by_tactic (0 + 1 + a + b + c + d + 2 == (b + 0) + 2 + d + (c + a + 0) + 1)
+  (fun _ -> canon_monoid (equality_equiv int) int_plus_cm)
+
+open FStar.Mul
+
+let test2 =
+  assert_by_tactic (forall (a b c d : int). ((b + 1) * 1) * 2 * a * (c * a) * 1 == a * (b + 1) * c * a * 2)
+  (fun _ -> ignore (forall_intros()); canon_monoid (equality_equiv int) int_multiply_cm)
+*)
+
+
+
+/////////////////////////////////////////////
+
+(*
+open LowStar.Resource
+
+let req : equiv resource = 
+  EQ equal 
+     equal_refl 
+     equal_symm 
+     equal_trans
+
+let rm : cm resource req =
+  CM empty_resource 
+     (<*>) 
+     equal_comm_monoid_left_unit 
+     equal_comm_monoid_associativity 
+     equal_comm_monoid_commutativity 
+     equal_comm_monoid_cong
+
+let compute_delta (outer inner:term) : Tac unit =
+
+  //introducing the refinement
+  refine_intro ();
+
+  dump "after refine_intro";
+
+  flip ();
+
+  dump "after flip";
+
+  canon_monoid req rm;
+
+  dump "after canon_monoid";
+
+  admit1 ()
+
+
+let test (outer inner:resource) 
+         (#[compute_delta (quote outer) (quote inner)] delta:resource{outer `equal` (inner <*> delta)})
+  : resource = delta
+let _ = assert (test (empty_resource <*> empty_resource) (empty_resource) == empty_resource)
+*)
+
+/////////////////////////////////////////////
+
+
+
+
+
+
+
+(*
   match term_as_formula (cur_goal ()) with
   | Comp (Eq (Some t)) t1 t2 ->
       // dump ("t1 =" ^ term_to_string t1 ^
@@ -355,19 +472,7 @@ let canon_monoid (#a:Type) (eq:equiv a) (m:cm a eq) : Tac unit =
                 `%List.Tot.Base.partition; `%bool_of_compare; `%compare_of_bool;
                 `%EQ?.eq;
            ]; primops]
-        // ;apply (`monoid_reflexivity)
-        // ;dump "done"
+        //;dump "done"
       else fail "Goal should be an equality at the right monoid type"
   | _ -> fail "Goal should be an equality"
-
-(***** Example *)
-
-let lem0 (a b c d : int) =
-  assert_by_tactic (0 + 1 + a + b + c + d + 2 == (b + 0) + 2 + d + (c + a + 0) + 1)
-  (fun _ -> canon_monoid (equality_equiv int) int_plus_cm)
-
-open FStar.Mul
-
-let _ =
-  assert_by_tactic (forall (a b c d : int). ((b + 1) * 1) * 2 * a * (c * a) * 1 == a * (b + 1) * c * a * 2)
-  (fun _ -> ignore (forall_intros()); canon_monoid (equality_equiv int) int_multiply_cm)
+*)
